\begin{frame}{Ejemplo}
  Vamos a ver que $P_n(x)= 1 - x^2 + x^4 - x^6 \dots + (-1)^nx^{2n}$ es polinomio de Taylor de
  $f(x)= \frac{1}{1+x^2}$ en $x_0=0$.

  $$|\frac{1}{1+x^2}-(1 - x^2 + x^4 - x^6 \dots + (-1)^nx^{2n})|
  =$$$$|\frac{1-1-x^2+x^2+x^4-x^4 \dots (-1)^{n+1}x^{2n+2}}{1+x^2}|=|\frac{(-1)^{n+1}x^{2n+2}}{1+x^2}|$$
  Si $|x|< \frac{1}{2}$:
  $$|\frac{x^{2n+2}}{1+x^2}|\leq |\frac{x^{n+1}}{1+x^2}| \leq 2|x^{n+1}| $$

  Esta desigualdad nos garantiza que $P_n(x)$
  es una caracterizaciÃ³n
\end{frame}
